@prefix : <http://purl.org/lis590od/Fall17/OrgRel#> .
@prefix dc: <http://purl.org/dc/elements/1.1/> .
@prefix tl: <http://purl.org/NET/c4dm/timeline.owl#> .
@prefix dbp: <http://dbpedia.org/resource/> .
@prefix geo: <http://www.w3.org/2003/01/geo/wgs84_pos#> .
@prefix org: <http://www.w3.org/ns/org#> .
@prefix owl: <http://www.w3.org/2002/07/owl#> .
@prefix rdf: <http://www.w3.org/1999/02/22-rdf-syntax-ns#> .
@prefix xml: <http://www.w3.org/XML/1998/namespace> .
@prefix xsd: <http://www.w3.org/2001/XMLSchema#> .
@prefix xsp: <http://www.owl-ontologies.com/2005/08/07/xsp.owl#> .
@prefix foaf: <http://xmlns.com/foaf/0.1/> .
@prefix prov: <http://www.w3.org/ns/prov#> .
@prefix rdfs: <http://www.w3.org/2000/01/rdf-schema#> .
@prefix skos: <http://www.w3.org/2004/02/skos/core#> .
@prefix swrl: <http://www.w3.org/2003/11/swrl#> .
@prefix wped: <http://en.wikipedia.org/wiki/> .
@prefix dolce: <http://ontology.ip.rm.cnr.it/ontologies/DOLCE-Lite#> .
@prefix event: <http://purl.org/NET/c4dm/event.owl#> .
@prefix swrlb: <http://www.w3.org/2003/11/swrlb#> .
@prefix dcterms: <http://purl.org/dc/terms/> .
@prefix protege: <http://protege.stanford.edu/plugins/owl/protege#> .

<http://purl.org/lis590od/Fall17/OrgRel> a owl:Ontology ;
	owl:imports <http://purl.org/NET/c4dm/event.owl> , <http://xmlns.com/foaf/0.1/> .
# 
# 
# #################################################################
# #
# #    Object Properties
# #
# #################################################################
# 
# 
# http://purl.org/lis590od/Fall17/OrgRel#agency

:agency a owl:ObjectProperty ;
	rdfs:domain :OrganizationRelationship ;
	rdfs:range foaf:Organization ;
	rdfs:comment "The organization or agency with which a person is involed in a time-bounded relationship"@en ;
	rdfs:label "agency"@en .
# 
# http://purl.org/lis590od/Fall17/OrgRel#agencyRole

:agencyRole a owl:ObjectProperty ;
	rdfs:domain :OrganizationRelationship ;
	rdfs:range skos:Concept ;
	rdfs:comment "The nature or type of relationship that an organization has with a person."@en ;
	rdfs:label "agency role"@en .
# 
# http://purl.org/lis590od/Fall17/OrgRel#client

:client a owl:ObjectProperty ;
	rdfs:domain :OrganizationRelationship ;
	rdfs:range foaf:Person ;
	rdfs:comment "The person involved in a relationship with an organization or agency"@en .
# 
# http://purl.org/lis590od/Fall17/OrgRel#clientRole

:clientRole a owl:ObjectProperty ;
	rdfs:domain :OrganizationRelationship ;
	rdfs:range skos:Concept ;
	rdfs:comment "The nature or type of relationship that a person has with an organization or agency"@en ;
	rdfs:label "client role"@en .
# 
# 
# 
# #################################################################
# #
# #    Classes
# #
# #################################################################
# 
# 
# http://purl.org/lis590od/Fall17/OrgRel#OrganizationRelationship

:OrganizationRelationship a owl:Class ;
	rdfs:subClassOf event:Event ;
	rdfs:label "Organization Relationship" .
# 
# Generated by the OWL API (version 4.1.3.20151118-2017) https://github.com/owlcs/owlapi
